#+AUTHOR: Ryan Sharif, 204-351-724
#+TITLE: CS180: Homework 2 | Section 1B
#+OPTIONS: toc:nil
#+LATEX_HEADER: \usepackage{amsthm}
#+LATEX_HEADER: \usepackage{mathtools}

* Glass jars

* Wires

* Problem 3

* Crossing a rickety bridge

* Induction

** The sum of the first $n$ integers is $\frac{n(n+1)}{2}$
   \begin{proof}
   The sum of the first $n$ integers is $\frac{n(n+1)}{2}$
   
   We will use a proof by induction. First, let us begin with the base case
   where $n = 1$. We check to see if the statement holds:

   \begin{align*}
   f(1) &= \frac{1(1+1)}{2} \\
   &= \frac{2}{2} \\
   &= 1
   \end{align*}

   Since, this holds true for our base case, we can make the inductive
   assumption, that is th  sum of the first $n$ integers
   is $\frac{n(n+1)}{2}$. Now we show that this holds for $n + 1$:

   \begin{align*}
   1 + 2 + 3 + ... + n + (n + 1) &= \frac{(n+1)(n+2)}{2} \\
   \shortintertext{Using our inductive assumption, we know the sum of
   of the first $n$ numbers}
   \frac{n(n+1)}{2} + n +1 &= \\
   \frac{n(n+1)+2(n+1)}{2} &= \\
   \frac{n(n+1)+2n + 2}{2} &= \\
   \frac{n^2 + n + 2n + 2}{2} &= \\
   \frac{n^2 + 3n + 2}{2} &= \\
   \frac{(n+1)(n+2)}{2} &= \frac{(n+1)(n+2)}{2}
   \end{align*}
   Thus, since we have shown that our left hand side is equivalent to
   the right hand side, we have shown what we wanted to prove.
   
   \end{proof}

** Inductive proof 2
\begin{proof}
$1\cdot2 + 2\cdot3 + 3\cdot4 + ... +n(n+1) = \frac{n(n+1)(n+2)}{3}$

Let us begin our proof by showing that the base case, where $n = 1$ holds:

\begin{align*}
f(1) = 1 \cdot 2 &= \frac{1(1+1)(1+2)}{3}\\
&= \frac{6}{3} \\
&= 2
\end{align*}

Since our base case obtains, we can make the inductive assumption and show
that for any $n$, our statement holds:

\begin{align*}
  1\cdot2 + 2\cdot3 + 3\cdot4 + ... +n(n+1) + n(n+2) &= \frac{(n+1)(n+2)(n+3)}{3} \\
  \frac{n(n+1)(n+2)}{3} + (n+1)(n+2) &= \\
  \frac{n(n+1)(n+2)+3(n+1)(n+2)}{3} &= \\
  \frac{(n+1)(n+2)(n+3)}{3} &=  \frac{(n+1)(n+2)(n+3)}{3}
\end{align*}

\end{proof}
